uniqueHeap/Heap.v
@@ -247,3 +247,39 @@ Proof.
   intros. destruct H. simpl in *. eapply rawHeapsEq. apply raw_replaceOverwrite. 
 Qed. 
 
+Theorem ltLookup : forall T u x H v, raw_heap_lookup x H = Some v ->
+                                       monotonic u T H -> optLT x u = true. 
+Proof.
+  induction H; intros. 
+  {inv H. }
+  {simpl in *. destruct a. destruct (beq_nat x i) eqn:eq. 
+   {inv H0. inversion H1; subst. apply beq_nat_true in eq. subst; auto. }
+   {eapply IHlist; eauto. inversion H1; subst. eapply monotonicLowerUB; eauto. }
+  }
+Qed. 
+
+Theorem raw_lookupReplaceSwitch : forall T x x' (v v':T) H,
+                                x<>x' -> raw_replace x v (raw_replace x' v' H) =
+                                         raw_replace x' v' (raw_replace x v H).
+Proof.
+  induction H. 
+  {auto. }
+  {intros. simpl. destruct a. destruct(beq_nat x' i) eqn:eq1. 
+   {destruct(beq_nat x i) eqn:eq2. 
+    {apply beq_nat_true in eq1. apply beq_nat_true in eq2. subst. exfalso; apply H0; auto. }
+    {simpl. apply beq_nat_false_iff in H0. rewrite H0. rewrite eq1. auto. }
+   }
+   {destruct (beq_nat x i) eqn:eq2. 
+    {simpl. rewrite eq2. apply beq_nat_false_iff in H0. destruct (beq_nat x' x) eqn:eq3; auto. 
+     apply beq_nat_true in eq3. subst. apply beq_nat_false in H0. exfalso. apply H0; auto. }
+    {simpl. rewrite eq1. rewrite eq2. rewrite IHlist. auto. assumption. }
+   }
+  }
+Qed.  
+
+Theorem lookupReplaceSwitch : forall T x x' (v v':T) H,
+                                x<>x' -> replace x v (replace x' v' H) = replace x' v' (replace x v H).
+Proof.
+  intros. destruct H; simpl in *. apply rawHeapsEq. apply raw_lookupReplaceSwitch; auto. 
+Qed. 
+
