uniqueHeap/nonspeculativeImpliesSpeculative.v
@@ -7,7 +7,8 @@ Require Import Coq.Sets.Ensembles.
 Require Import sets. 
 Require Import Powerset_facts. 
 Require Import erasure. 
-
+Require Import SpecLib. 
+Require Import unspec. 
 
 (*terms that when erased to require the erased thread to be commit*)
 Inductive commitTrm : ptrm -> Prop :=
@@ -25,52 +26,43 @@ Ltac commitFill :=
      eapply pctxtUnique in H; eauto; inversion H as [Eq1 Eq2]; inversion Eq2
   end. 
 
+Ltac existTac e := let n := fresh in
+                   try(assert(n:exists e', eraseTerm e' = e) by apply eTerm; invertHyp);
+                   try(assert(n:exists e', eraseCtxt e' = e) by apply eCtxt; invertHyp). 
+
+
 Theorem eraseThreadCommitTrm : forall x t, commitTrm t -> eraseThread x (pSingleton t) ->
                                        exists tid s2 M, x = (tid,nil,s2,M) /\ eraseTerm M = t.
 Proof.
   intros. inversion H0; subst. 
   {exists tid. exists s2. exists M. split; auto. apply SingletonEq in H3. subst. auto. }
-  {apply SingletonEq in H1; subst. copy H4. apply decomposeEq in H4. subst. rewrite eraseFill in H. 
-   inversion H; subst; try solve[
-   commitFill; clear H;[
-    match goal with
-        |H:decompose ?t ?E ?e |- _ => apply pdecomposeDecomposed; try constructor;
-                                      apply decomposeWF in H; apply eraseCtxtWF; auto
-    end| commitFill]]. destruct (eraseCtxt E); simpl in H3; inversion H3. }
-  {apply SingletonEq in H1; subst. copy H4. apply decomposeEq in H4. subst. rewrite eraseFill in H. 
-   inversion H; subst; try solve[
-   commitFill; clear H;[
-    match goal with
-        |H:decompose ?t ?E ?e |- _ => apply pdecomposeDecomposed; try constructor;
-                                      apply decomposeWF in H; apply eraseCtxtWF; auto
-    end| commitFill]]. destruct (eraseCtxt E); simpl in H3; inversion H3. }
-  {apply SingletonEq in H1; subst. copy H4. apply decomposeEq in H4. subst. rewrite eraseFill in H. 
-   inversion H; subst; try solve[
-   commitFill; clear H;[
-    match goal with
-        |H:decompose ?t ?E ?e |- _ => apply pdecomposeDecomposed; try constructor;
-                                      apply decomposeWF in H; apply eraseCtxtWF; auto
-    end| commitFill]]. destruct (eraseCtxt E); simpl in H3; inversion H3. }
-  {apply SingletonEq in H1; subst. copy H4. apply decomposeEq in H4. subst. rewrite eraseFill in H. 
-   inversion H; subst; try solve[
-   commitFill; clear H;[
-    match goal with
-        |H:decompose ?t ?E ?e |- _ => apply pdecomposeDecomposed; try constructor;
-                                      apply decomposeWF in H; apply eraseCtxtWF; auto
-    end| commitFill]]. destruct (eraseCtxt E); simpl in H3; inversion H3. }
-  {apply SingletonEq in H1; subst. copy H4. apply decomposeEq in H4. subst. rewrite eraseFill in H. 
-   inversion H; subst; try solve[
-   commitFill; clear H;[
-    match goal with
-        |H:decompose ?t ?E ?e |- _ => apply pdecomposeDecomposed; try constructor;
-                                      apply decomposeWF in H; apply eraseCtxtWF; auto
-    end| commitFill]]. destruct (eraseCtxt E); simpl in H3; inversion H3. }
-  {symmetry in H1. apply SingletonNeqEmpty in H1. inversion H1. }
-Qed. 
-
-Ltac eErase e := try (assert(exists e', eraseTerm e' = e) by apply eTerm; invertHyp);
-                try (assert(exists e', eraseCtxt e' = e) by apply eCtxt; invertHyp);
-                try(assert(exists e', eraseThread e' e) by apply eThread; invertHyp).
+  {unfold pSingleton in *; invertHyp. inv H; try(copy d;
+   match goal with
+       |H:pdecompose ?M ?E ?e, H':decompose ?M' ?E' ?e' |- _ => 
+        rewrite <- decomposeErase in H'; eauto; eapply pctxtUnique in H; eauto; invertHyp 
+   end; inv H3). destruct M'; inv H2. inv d. }
+  {unfold pSingleton in *; invertHyp. inv H; try(copy d;
+   match goal with
+       |H:pdecompose ?M ?E ?e, H':decompose ?M' ?E' ?e' |- _ => 
+        rewrite <- decomposeErase in H'; eauto; eapply pctxtUnique in H; eauto; invertHyp 
+   end; inv H3). destruct M'; inv H2. inv d. }
+  {unfold pSingleton in *; invertHyp. inv H; try(copy d;
+   match goal with
+       |H:pdecompose ?M ?E ?e, H':decompose ?M' ?E' ?e' |- _ => 
+        rewrite <- decomposeErase in H'; eauto; eapply pctxtUnique in H; eauto; invertHyp 
+   end; inv H3). destruct M'; inv H2. inv d. }
+  {unfold pSingleton in *; invertHyp. inv H; try(copy d;
+   match goal with
+       |H:pdecompose ?M ?E ?e, H':decompose ?M' ?E' ?e' |- _ => 
+        rewrite <- decomposeErase in H'; eauto; eapply pctxtUnique in H; eauto; invertHyp 
+   end; inv H3). destruct M'; inv H2. inv d. }
+  {unfold pSingleton in *; invertHyp. inv H; try(copy d;
+   match goal with
+       |H:pdecompose ?M ?E ?e, H':decompose ?M' ?E' ?e' |- _ => 
+        rewrite <- decomposeErase in H'; eauto; eapply pctxtUnique in H; eauto; invertHyp 
+   end; inv H3). destruct M'; inv H2. inv d. }
+  {symmetry in H1. apply SingletonNeqEmpty in H1. inv H1. }
+Qed.
 
 Theorem erasePoolSingleton : forall T t', erasePoolAux T = pSingleton t' ->
                                           exists t, tIn T t /\ eraseThread t (pSingleton t'). 
@@ -78,17 +70,44 @@ Proof.
   intros. apply eqImpliesSameSet in H. unfold Same_set in H. unfold Included in H. inv H. 
   assert(In ptrm (pSingleton t') t'). constructor. apply H1 in H. inv H. inv H2. inv H5.
   inv H3; try solve[econstructor; split; eauto; inv H4; eauto]. Qed. 
- 
+
+Theorem eraseThreadCardinality : forall t t', eraseThread t t' -> 
+                                              t' = Empty_set ptrm \/ exists t'', t' = pSingleton t''.
+Proof.
+  intros. inv H; eauto. 
+Qed. 
+
 Theorem nonspecImpliesSpec' : forall PH PH' PT pt pt' H T,
                                pstep PH PT pt (pOK PH' PT pt') -> eraseHeap H = PH ->
                                erasePool T (Union ptrm PT pt) ->
                                exists H' T' t' t'',
                                  T = tUnion T' t' /\ 
                                  eraseHeap H' = PH' /\ erasePool (tUnion T' t'') (Union ptrm PT pt') /\
-                                 multistep H T' t' (OK H' T' t'). 
+                                 multistep H T' t' (OK H' T' t''). 
 Proof.
   intros. inversion H0; subst. 
-  {exists H. inversion H2; subst. 
+  {exists H. inversion H2; subst. unfoldSetEq H5. assert(In ptrm (pUnion PT (pSingleton t)) t). 
+   apply Union_intror. constructor. apply H3 in H4. inversion H4; subst. inv H5. 
+   inv H10. apply pullOut in H9. rewrite H9 in H2. exists (Subtract thread T(t0,s0,s3,M0)). 
+   exists (tSingleton(t0,s0,s3,M0)). existTac E. existTac e. existTac arg. econstructor.
+   split. auto. split; auto. clear H9. inv H2. rewrite eraseUnionComm in H13. 
+   copy H6. apply eraseThreadCardinality in H6. inv H6. inv H8. invertHyp. inv H8. 
+   eapply eraseThreadCommitTrm in H2; eauto. invertHyp. Focus 2. eapply commitApp; eauto.
+   inv H2. split. Focus 2. eapply multi_step. rewrite <- union_empty_l at 1. auto. 
+   eapply BetaRed. eapply decomposeErase in H7; eauto. simpl; auto. constructor. 
+   
+
+
+
+econstructor. split; auto. split; auto. clear H9. inv H2. 
+   rewrite eraseUnionComm in H10. copy H6. apply eraseThreadCardinality in H6. inv H6. 
+   inv H8. invertHyp. inv H8. eapply eraseThreadCommitTrm in H2; eauto. Focus 2. 
+   eapply commitApp; eauto. invertHyp. inv H2. existTac E. existTac e. existTac arg. 
+   split. Focus 2. eapply multi_step. rewrite <- union_empty_l at 1. auto. eapply BetaRed. 
+   eapply decomposeErase in H7; eauto. simpl. auto. unfoldTac. rewrite union_empty_l. 
+   apply multi_refl. constructor. 
+
+
 
 Theorem ePool : forall T', exists T, erasePool T T'.
 Admitted.  
